theories/AutoSubst/Ast.v
@@ -10,7 +10,7 @@ Inductive term : Type :=
   | tSort : sort -> term
   | tProd : term -> term -> term
   | tLambda : term -> term -> term
-  | tApp : term -> term -> term
+  | tApp : term -> term -> term -> term -> term
   | tNat : term
   | tZero : term
   | tSucc : term -> term
@@ -45,11 +45,16 @@ exact (eq_trans (eq_trans eq_refl (ap (fun x => tLambda x s1) H0))
          (ap (fun x => tLambda t0 x) H1)).
 Qed.
 
-Lemma congr_tApp {s0 : term} {s1 : term} {t0 : term} {t1 : term}
-  (H0 : s0 = t0) (H1 : s1 = t1) : tApp s0 s1 = tApp t0 t1.
+Lemma congr_tApp {s0 : term} {s1 : term} {s2 : term} {s3 : term} {t0 : term}
+  {t1 : term} {t2 : term} {t3 : term} (H0 : s0 = t0) (H1 : s1 = t1)
+  (H2 : s2 = t2) (H3 : s3 = t3) : tApp s0 s1 s2 s3 = tApp t0 t1 t2 t3.
 Proof.
-exact (eq_trans (eq_trans eq_refl (ap (fun x => tApp x s1) H0))
-         (ap (fun x => tApp t0 x) H1)).
+exact (eq_trans
+         (eq_trans
+            (eq_trans (eq_trans eq_refl (ap (fun x => tApp x s1 s2 s3) H0))
+               (ap (fun x => tApp t0 x s2 s3) H1))
+            (ap (fun x => tApp t0 t1 x s3) H2))
+         (ap (fun x => tApp t0 t1 t2 x) H3)).
 Qed.
 
 Lemma congr_tNat : tNat = tNat.
@@ -172,7 +177,9 @@ Fixpoint ren_term (xi_term : nat -> nat) (s : term) {struct s} : term :=
       tProd (ren_term xi_term s0) (ren_term (upRen_term_term xi_term) s1)
   | tLambda s0 s1 =>
       tLambda (ren_term xi_term s0) (ren_term (upRen_term_term xi_term) s1)
-  | tApp s0 s1 => tApp (ren_term xi_term s0) (ren_term xi_term s1)
+  | tApp s0 s1 s2 s3 =>
+      tApp (ren_term xi_term s0) (ren_term (upRen_term_term xi_term) s1)
+        (ren_term xi_term s2) (ren_term xi_term s3)
   | tNat => tNat
   | tZero => tZero
   | tSucc s0 => tSucc (ren_term xi_term s0)
@@ -215,7 +222,10 @@ term :=
   | tLambda s0 s1 =>
       tLambda (subst_term sigma_term s0)
         (subst_term (up_term_term sigma_term) s1)
-  | tApp s0 s1 => tApp (subst_term sigma_term s0) (subst_term sigma_term s1)
+  | tApp s0 s1 s2 s3 =>
+      tApp (subst_term sigma_term s0)
+        (subst_term (up_term_term sigma_term) s1) (subst_term sigma_term s2)
+        (subst_term sigma_term s3)
   | tNat => tNat
   | tZero => tZero
   | tSucc s0 => tSucc (subst_term sigma_term s0)
@@ -270,9 +280,11 @@ subst_term sigma_term s = s :=
   | tLambda s0 s1 =>
       congr_tLambda (idSubst_term sigma_term Eq_term s0)
         (idSubst_term (up_term_term sigma_term) (upId_term_term _ Eq_term) s1)
-  | tApp s0 s1 =>
+  | tApp s0 s1 s2 s3 =>
       congr_tApp (idSubst_term sigma_term Eq_term s0)
-        (idSubst_term sigma_term Eq_term s1)
+        (idSubst_term (up_term_term sigma_term) (upId_term_term _ Eq_term) s1)
+        (idSubst_term sigma_term Eq_term s2)
+        (idSubst_term sigma_term Eq_term s3)
   | tNat => congr_tNat
   | tZero => congr_tZero
   | tSucc s0 => congr_tSucc (idSubst_term sigma_term Eq_term s0)
@@ -338,9 +350,12 @@ ren_term xi_term s = ren_term zeta_term s :=
       congr_tLambda (extRen_term xi_term zeta_term Eq_term s0)
         (extRen_term (upRen_term_term xi_term) (upRen_term_term zeta_term)
            (upExtRen_term_term _ _ Eq_term) s1)
-  | tApp s0 s1 =>
+  | tApp s0 s1 s2 s3 =>
       congr_tApp (extRen_term xi_term zeta_term Eq_term s0)
-        (extRen_term xi_term zeta_term Eq_term s1)
+        (extRen_term (upRen_term_term xi_term) (upRen_term_term zeta_term)
+           (upExtRen_term_term _ _ Eq_term) s1)
+        (extRen_term xi_term zeta_term Eq_term s2)
+        (extRen_term xi_term zeta_term Eq_term s3)
   | tNat => congr_tNat
   | tZero => congr_tZero
   | tSucc s0 => congr_tSucc (extRen_term xi_term zeta_term Eq_term s0)
@@ -412,9 +427,12 @@ subst_term sigma_term s = subst_term tau_term s :=
       congr_tLambda (ext_term sigma_term tau_term Eq_term s0)
         (ext_term (up_term_term sigma_term) (up_term_term tau_term)
            (upExt_term_term _ _ Eq_term) s1)
-  | tApp s0 s1 =>
+  | tApp s0 s1 s2 s3 =>
       congr_tApp (ext_term sigma_term tau_term Eq_term s0)
-        (ext_term sigma_term tau_term Eq_term s1)
+        (ext_term (up_term_term sigma_term) (up_term_term tau_term)
+           (upExt_term_term _ _ Eq_term) s1)
+        (ext_term sigma_term tau_term Eq_term s2)
+        (ext_term sigma_term tau_term Eq_term s3)
   | tNat => congr_tNat
   | tZero => congr_tZero
   | tSucc s0 => congr_tSucc (ext_term sigma_term tau_term Eq_term s0)
@@ -487,9 +505,13 @@ Fixpoint compRenRen_term (xi_term : nat -> nat) (zeta_term : nat -> nat)
         (compRenRen_term (upRen_term_term xi_term)
            (upRen_term_term zeta_term) (upRen_term_term rho_term)
            (up_ren_ren _ _ _ Eq_term) s1)
-  | tApp s0 s1 =>
+  | tApp s0 s1 s2 s3 =>
       congr_tApp (compRenRen_term xi_term zeta_term rho_term Eq_term s0)
-        (compRenRen_term xi_term zeta_term rho_term Eq_term s1)
+        (compRenRen_term (upRen_term_term xi_term)
+           (upRen_term_term zeta_term) (upRen_term_term rho_term)
+           (up_ren_ren _ _ _ Eq_term) s1)
+        (compRenRen_term xi_term zeta_term rho_term Eq_term s2)
+        (compRenRen_term xi_term zeta_term rho_term Eq_term s3)
   | tNat => congr_tNat
   | tZero => congr_tZero
   | tSucc s0 =>
@@ -575,9 +597,12 @@ subst_term tau_term (ren_term xi_term s) = subst_term theta_term s :=
         (compRenSubst_term (upRen_term_term xi_term) (up_term_term tau_term)
            (up_term_term theta_term) (up_ren_subst_term_term _ _ _ Eq_term)
            s1)
-  | tApp s0 s1 =>
+  | tApp s0 s1 s2 s3 =>
       congr_tApp (compRenSubst_term xi_term tau_term theta_term Eq_term s0)
-        (compRenSubst_term xi_term tau_term theta_term Eq_term s1)
+        (compRenSubst_term (upRen_term_term xi_term) (up_term_term tau_term)
+           (up_term_term theta_term) (up_ren_subst_term_term _ _ _ Eq_term)
+           s1) (compRenSubst_term xi_term tau_term theta_term Eq_term s2)
+        (compRenSubst_term xi_term tau_term theta_term Eq_term s3)
   | tNat => congr_tNat
   | tZero => congr_tZero
   | tSucc s0 =>
@@ -673,10 +698,14 @@ ren_term zeta_term (subst_term sigma_term s) = subst_term theta_term s :=
         (compSubstRen_term (up_term_term sigma_term)
            (upRen_term_term zeta_term) (up_term_term theta_term)
            (up_subst_ren_term_term _ _ _ Eq_term) s1)
-  | tApp s0 s1 =>
+  | tApp s0 s1 s2 s3 =>
       congr_tApp
         (compSubstRen_term sigma_term zeta_term theta_term Eq_term s0)
-        (compSubstRen_term sigma_term zeta_term theta_term Eq_term s1)
+        (compSubstRen_term (up_term_term sigma_term)
+           (upRen_term_term zeta_term) (up_term_term theta_term)
+           (up_subst_ren_term_term _ _ _ Eq_term) s1)
+        (compSubstRen_term sigma_term zeta_term theta_term Eq_term s2)
+        (compSubstRen_term sigma_term zeta_term theta_term Eq_term s3)
   | tNat => congr_tNat
   | tZero => congr_tZero
   | tSucc s0 =>
@@ -784,10 +813,14 @@ subst_term tau_term (subst_term sigma_term s) = subst_term theta_term s :=
         (compSubstSubst_term (up_term_term sigma_term)
            (up_term_term tau_term) (up_term_term theta_term)
            (up_subst_subst_term_term _ _ _ Eq_term) s1)
-  | tApp s0 s1 =>
+  | tApp s0 s1 s2 s3 =>
       congr_tApp
         (compSubstSubst_term sigma_term tau_term theta_term Eq_term s0)
-        (compSubstSubst_term sigma_term tau_term theta_term Eq_term s1)
+        (compSubstSubst_term (up_term_term sigma_term)
+           (up_term_term tau_term) (up_term_term theta_term)
+           (up_subst_subst_term_term _ _ _ Eq_term) s1)
+        (compSubstSubst_term sigma_term tau_term theta_term Eq_term s2)
+        (compSubstSubst_term sigma_term tau_term theta_term Eq_term s3)
   | tNat => congr_tNat
   | tZero => congr_tZero
   | tSucc s0 =>
@@ -943,9 +976,12 @@ Fixpoint rinst_inst_term (xi_term : nat -> nat) (sigma_term : nat -> term)
       congr_tLambda (rinst_inst_term xi_term sigma_term Eq_term s0)
         (rinst_inst_term (upRen_term_term xi_term) (up_term_term sigma_term)
            (rinstInst_up_term_term _ _ Eq_term) s1)
-  | tApp s0 s1 =>
+  | tApp s0 s1 s2 s3 =>
       congr_tApp (rinst_inst_term xi_term sigma_term Eq_term s0)
-        (rinst_inst_term xi_term sigma_term Eq_term s1)
+        (rinst_inst_term (upRen_term_term xi_term) (up_term_term sigma_term)
+           (rinstInst_up_term_term _ _ Eq_term) s1)
+        (rinst_inst_term xi_term sigma_term Eq_term s2)
+        (rinst_inst_term xi_term sigma_term Eq_term s3)
   | tNat => congr_tNat
   | tZero => congr_tZero
   | tSucc s0 => congr_tSucc (rinst_inst_term xi_term sigma_term Eq_term s0)
@@ -1064,28 +1100,28 @@ Class Up_term X Y :=
 Instance VarInstance_term : (Var _ _) := @tRel.
 
 Notation "[ sigma_term ]" := (subst_term sigma_term)
-  ( at level 1, left associativity, only printing) : fscope.
+( at level 1, left associativity, only printing)  : fscope.
 
 Notation "s [ sigma_term ]" := (subst_term sigma_term s)
-  ( at level 7, left associativity, only printing) : subst_scope.
+( at level 7, left associativity, only printing)  : subst_scope.
 
-Notation "↑__term" := up_term (only printing) : subst_scope.
+Notation "↑__term" := up_term (only printing)  : subst_scope.
 
-Notation "↑__term" := up_term_term (only printing) : subst_scope.
+Notation "↑__term" := up_term_term (only printing)  : subst_scope.
 
 Notation "⟨ xi_term ⟩" := (ren_term xi_term)
-  ( at level 1, left associativity, only printing) : fscope.
+( at level 1, left associativity, only printing)  : fscope.
 
 Notation "s ⟨ xi_term ⟩" := (ren_term xi_term s)
-  ( at level 7, left associativity, only printing) : subst_scope.
+( at level 7, left associativity, only printing)  : subst_scope.
 
-Notation "'var'" := tRel ( at level 1, only printing) : subst_scope.
+Notation "'var'" := tRel ( at level 1, only printing)  : subst_scope.
 
 Notation "x '__term'" := (@ids _ _ VarInstance_term x)
-  ( at level 5, format "x __term", only printing) : subst_scope.
+( at level 5, format "x __term", only printing)  : subst_scope.
 
-Notation "x '__term'" := (tRel x) ( at level 5, format "x __term") :
-  subst_scope.
+Notation "x '__term'" := (tRel x) ( at level 5, format "x __term")  :
+subst_scope.
 
 #[global]
 Instance subst_term_morphism :
