theories/ParallelRed.v
@@ -1,0 +1,427 @@
+(** * LogRel.ParallelRed: definition of parallel reduction. *)
+From Coq Require Import ssreflect.
+From smpl Require Import Smpl.
+From LogRel.AutoSubst Require Import core unscoped Ast Extra.
+From LogRel Require Import Utils BasicAst Notations Context NormalForms Weakening.
+From LogRel Require Import GenericTyping.
+
+Set Primitive Projections.
+
+Class EqType (ta : tag) := eq_type : context -> term -> term -> Set.
+Class EqTerm (ta : tag) := eq_term : context -> term -> term -> term -> Set.
+
+Notation "[ Γ |- A = B ]" := (eq_type Γ A B)
+  (at level 0, Γ, A, B at level 50, only parsing) : typing_scope.
+  Notation "[ Γ |-[ ta  ] A = B ]" := (eq_type (ta := ta) Γ A B)
+    (at level 0, Γ, A, B at level 50) : typing_scope.
+Notation "[ Γ |- t = u : A ]" := (eq_term Γ A t u)
+  (at level 0, Γ, A, t, u at level 50, only parsing) : typing_scope.
+Notation "[ Γ |-[ ta  ] t = u : A ]" := (eq_term (ta := ta) Γ A t u)
+  (at level 0, Γ, A, t, u at level 50) : typing_scope.
+  
+
+(** ** Definitions *)
+Section Definitions.
+
+  (* We locally disable typing notations to be able to use them in the definition
+  here before declaring the instance to which abstract notations are bound. *)
+  Close Scope typing_scope.
+
+
+  (** Reduction and conversion are mutually defined inductive relations. Typing is just a
+    shortcut for a type reduction to itself. *)
+
+  (** **** Context well-formation *)
+  Inductive WfContextPar : context -> Type :=
+      | ConParNil : [ |- ε ]
+      | ConParCons {Γ A} : 
+          [ |- Γ ] -> 
+          [ Γ |- A ] -> 
+          [ |-  Γ ,, A]
+  (** **** Type  *)
+  with TypePar  : context -> term -> term -> Type :=
+      | TypeParU {Γ} : 
+          [ |- Γ ] ->
+          [ Γ |- U ⤳ U] 
+      | TypeParProd {Γ} {A A' B B'} :
+          [ Γ |- A ⤳ A'] -> 
+          [Γ ,, A |- B ⤳ B'] -> 
+          [ Γ |- tProd A B ⤳ tProd A' B']
+      | TypeParUniv {Γ} {A A'} :
+          [ Γ |- A ⤳ A' : U ] -> 
+          [ Γ |- A ⤳ A']
+  (** **** Typing *)
+  with TermPar : context -> term -> term -> term -> Type :=
+      | TermParVar {Γ} {n decl} :
+          [   |- Γ ] ->
+          in_ctx Γ n decl ->
+          [ Γ |- tRel n ⤳ tRel n : decl ]
+      | TermParProd {Γ} {A A' B B'} :
+          [ Γ |- A ⤳ A' : U] -> 
+          [Γ ,, A |- B ⤳ B' : U] -> 
+          [ Γ |- tProd A B ⤳ tProd A' B' : U]
+      | TermParLam {Γ} {A A' A'' B t t'} :
+          [Γ |- A ≅ A''] ->
+          [ Γ |- A ⤳ A' ] ->
+          [ Γ ,, A |- t ⤳ t' : B ] -> 
+          [ Γ |- tLambda A t ⤳ tLambda A' t' : tProd A'' B]
+      | TermParBeta {Γ} {A A' B a a' t t'} :
+          [Γ |- A] ->
+          [ Γ |- A' ≅ A] ->
+          [Γ ,, A |- B] ->
+          [ Γ ,, A' |- t ⤳ t' : B ] ->
+          [ Γ |- a ⤳ a' : A ] ->
+          [ Γ |- tApp A B (tLambda A' t) a ⤳ t'[a'..] : B[a..] ]
+      | TermParApp {Γ} {f f' a a' A A' B B'} :
+          [Γ |- A] ->
+          [Γ |- A ⤳ A' ] ->
+          [Γ,, A |- B] ->
+          [Γ,, A |- B ⤳ B'] ->
+          [ Γ |- f ⤳ f' : tProd A B ] -> 
+          [ Γ |- a ⤳ a' : A ] -> 
+          [ Γ |- tApp A B f a ⤳ tApp A' B' f' a' : B[a..] ]
+      | TermParConv {Γ} {A B t t'} :
+          [ Γ |- t ⤳ t' : A ] -> 
+          [ Γ |- A ≅ B ] -> 
+          [ Γ |- t ⤳ t' : B ]
+
+  (** **** Structural equality of types *)
+  with TypeEqPar : context -> term -> term  -> Type :=
+    | TypeEqParU {Γ} :
+        [ |- Γ ] ->
+        [ Γ |- U = U]
+      | TypeEqParProd {Γ} {A B C D} :
+          [ Γ |- A = B] ->
+          [ Γ ,, A |- C = D] ->
+          [ Γ |- tProd A C = tProd B D]
+      | TypeEqParUniv {Γ} {A B} :
+        [ Γ |- A = B : U ] -> 
+        [ Γ |- A = B ]
+
+  (** **** Structural equality of terms *)
+  with TermEqPar : context -> term -> term -> term -> Type :=
+      | TermEqParVar {Γ} {n decl} :
+        [   |- Γ ] ->
+        in_ctx Γ n decl ->
+        [ Γ |- tRel n = tRel n : decl ]
+      | TermEqParProd {Γ} {A A' B B'} :
+        [ Γ |- A = A' : U] -> 
+        [Γ ,, A |- B = B' : U] -> 
+        [ Γ |- tProd A B = tProd A' B' : U]
+      | TermEqParLam {Γ} {A A' A'' B t t'} :
+        [ Γ |- A ≅ A' ] ->
+        [Γ |- A ≅ A'' ] ->
+        [ Γ ,, A |- t = t' : B ] -> 
+        [ Γ |- tLambda A t = tLambda A' t' : tProd A'' B]
+      | TermEqParApp {Γ} {f f' a a' A A' B B'} :
+        [Γ |- A ≅ A' ] ->
+        [Γ,, A |- B ≅ B'] ->
+        [ Γ |- f = f' : tProd A B ] -> 
+        [ Γ |- a = a' : A ] -> 
+        [ Γ |- tApp A B f a = tApp A' B' f' a' : B[a..] ]
+      | TermEqParConv {Γ} {A B t t'} :
+        [ Γ |- t = t' : A ] -> 
+        [ Γ |- A ≅ B ] -> 
+        [ Γ |- t = t' : B ]
+
+  with TypeConvPar : context -> term -> term  -> Type :=
+      | TypeConvParEq {Γ A B} :
+          [ Γ |- A = B] ->
+          [ Γ |- A ≅ B]
+      | TypeConvParL {Γ} {A A' B} :
+          [ Γ |- A ⤳ A' ] ->
+          [ Γ |- A' ≅ B] ->
+          [ Γ |- A ≅ B ]
+      | TypeConvParR {Γ} {A B B'} :
+          [ Γ |- B ⤳ B' ] ->
+          [ Γ |- A ≅ B] ->
+          [ Γ |- A ≅ B ]
+
+  with TermConvPar : context -> term -> term -> term -> Type :=
+      | TermConvParEq {Γ A t u} :
+          [ Γ |- t = u : A] ->
+          [ Γ |- t ≅ u : A]
+      | TermConvParL {Γ} {A t t' u} :
+          [ Γ |- t ⤳ t' : A] ->
+          [ Γ |- t' ≅ u : A] ->
+          [ Γ |- t ≅ u : A]
+      | TermConvParR {Γ} {A t u u'} :
+          [ Γ |- u ⤳ u' : A] ->
+          [ Γ |- t ≅ u' : A] ->
+          [ Γ |- t ≅ u : A]
+      
+  where "[   |- Γ ]" := (WfContextPar Γ)
+  and   "[ Γ |- A ⤳ A' ]" := (TypePar Γ A A')
+  and   "[ Γ |- A ]" := (TypePar Γ A A)
+  and   "[ Γ |- t ⤳ t' : A ]" := (TermPar Γ A t t')
+  and   "[ Γ |- t : T ]" := (TermPar Γ T t t)
+  and   "[ Γ |- A = B ]" := (TypeEqPar Γ A B)
+  and   "[ Γ |- t = t' : T ]" := (TermEqPar Γ T t t')
+  and   "[ Γ |- A ≅ B ]" := (TypeConvPar Γ A B)
+  and   "[ Γ |- t ≅ t' : T ]" := (TermConvPar Γ T t t').
+
+  Inductive TermParClos (Γ : context) (A : term) : term -> term -> Type :=
+    | TermParRedRefl t : [Γ |- t : A] -> [Γ |- t ⤳* t : A]
+    | TermParRedTrans t t' t'' : [Γ |- t ⤳ t' : A] -> [Γ |- t' ⤳* t'' : A] -> [Γ |- t ⤳* t'' : A]
+  where "[ Γ |- t ⤳* t' : A ]" := (TermParClos Γ A t t').
+
+  Inductive TypeParClos (Γ : context) : term -> term -> Type :=
+    | TypeParRedRefl A : [Γ |- A ] -> [Γ |- A ⤳* A]
+    | TypeParRedTrans A A' A'' : [Γ |- A ⤳ A'] -> [Γ |- A' ⤳* A''] -> [Γ |- A ⤳* A'']
+  where "[ Γ |- A ⤳* A' ]" := (TypeParClos Γ A A').
+
+End Definitions.
+
+
+(** ** Instances *)
+(** Used for printing (see Notations) and as a support for the generic typing
+properties used for the logical relation (see GenericTyping). *)
+Module ParallelTypingData.
+
+  Definition pa : tag.
+  Proof.
+  constructor.
+  Qed.
+
+  #[export] Instance WfContext_Par : WfContext pa := WfContextPar.
+  #[export] Instance WfType_Par : WfType pa := fun Γ A => TypePar Γ A A.
+  #[export] Instance Typing_Par : Typing pa := fun Γ A t => TermPar Γ A t t.
+  #[export] Instance ConvType_Par : ConvType pa := TypeConvPar.
+  #[export] Instance ConvTerm_Par : ConvTerm pa := TermConvPar.
+  #[export] Instance EqType_Par : EqType pa := TypeEqPar.
+  #[export] Instance EqTerm_Par : EqTerm pa := TermEqPar.
+  #[export] Instance RedType_Par : RedType pa := TypeParClos.
+  #[export] Instance RedTerm_Par : RedTerm pa := TermParClos.
+  #[export] Instance OSRedType_Par : OneStepRedType pa := TypePar.
+  #[export] Instance OSRedTerm_Par : OneStepRedTerm pa := TermPar.
+
+  Ltac fold_pa :=
+    change WfContextPar with (wf_context (ta := pa)) in * ;
+    change (TypePar ?Γ ?A ?A) with (wf_type (ta := pa) Γ A) in * ;
+    change (TermPar ?Γ ?A ?t ?t) with (typing (ta := pa) Γ A t) in * ;
+    change TypeEqPar with (eq_type (ta := pa)) in * ;
+    change TermEqPar with (eq_term (ta := pa)) in * ;
+    change TypeConvPar with (conv_type (ta := pa)) in * ;
+    change TermConvPar with (conv_term (ta := pa)) in * ;
+    change TypeParClos with (red_ty (ta := pa)) in *;
+    change TermParClos with (red_tm (ta := pa)) in *;
+    change TypePar with (osred_ty (ta := pa)) in *;
+    change TermPar with (osred_tm (ta := pa)) in *.
+
+  Smpl Add fold_pa : refold.
+
+End ParallelTypingData.
+
+(** ** Induction principles *)
+
+(** We use Scheme to generate mutual induction principle. Sadly, Scheme uses
+the product of the standard library, which is not universe polymorphic, which
+causes universe issues, typically in the fundamental lemma. So
+we use some Ltac code to generate properly polymorphic versions of the inductive
+principle. We also use Ltac to generate the conclusion of the mutual induction
+proof, to alleviate the user from the need to write it down every time: they
+only need write the predicates to be proven. *)
+Section InductionPrinciples.
+  Import ParallelTypingData.
+
+Scheme 
+    Minimality for WfContextPar Sort Type with
+    Minimality for TypePar      Sort Type with
+    Minimality for TermPar      Sort Type with
+    Minimality for TypeEqPar    Sort Type with
+    Minimality for TermEqPar    Sort Type with
+    Minimality for TypeConvPar  Sort Type with
+    Minimality for TermConvPar  Sort Type.
+
+Combined Scheme _ParInduction from
+    WfContextPar_rect_nodep,
+    TypePar_rect_nodep,
+    TermPar_rect_nodep,
+    TypeEqPar_rect_nodep,
+    TermEqPar_rect_nodep,
+    TypeConvPar_rect_nodep,
+    TermConvPar_rect_nodep.
+
+Let _ParInductionType :=
+  ltac:(let ind := fresh "ind" in
+      pose (ind := _ParInduction);
+      refold ;
+      let ind_ty := type of ind in
+      exact ind_ty).
+
+Let ParInductionType :=
+  ltac: (let ind := eval cbv delta [_ParInductionType] zeta
+    in _ParInductionType in
+    let ind' := polymorphise ind in
+  exact ind').
+
+Lemma ParInduction : ParInductionType.
+Proof.
+  intros PCon PTy PTm PTyEq PTmEq PTyConv PTmConv **.
+  pose proof (_ParInduction PCon PTy PTm PTyEq PTmEq PTyConv PTmConv) as H.
+  destruct H as (?&?&?&?&?&?&?).
+  all: try (assumption ; fail).
+  repeat (split;[assumption|]); assumption.
+Qed.
+
+Definition ParInductionConcl :=
+  ltac:(
+    let t := eval cbv delta [ParInductionType] beta in ParInductionType in
+    let t' := remove_steps t in
+    exact t').
+
+End InductionPrinciples.
+
+Arguments ParInductionConcl PCon PTy PTm PTyEq PTmEq PTyConv PTmConv : rename.
+
+Import ParallelTypingData.
+
+Section LRefl.
+
+  Let PCon (Γ : context) := True.
+  Let PTy (Γ : context) (A A' : term) := [Γ |- A].
+  Let PTm (Γ : context) (A t t' : term) := [Γ |- t : A].
+  Let PTyEq (Γ : context) (A B : term) := [Γ |- A].
+  Let PTmEq (Γ : context) (A t u : term) := [Γ |- t : A].
+  Let PTyConv (Γ : context) (A B : term) := [Γ |- A].
+  Let PTmConv (Γ : context) (A t u : term) := [Γ |- t : A].
+
+  Theorem par_lrefl : ParInductionConcl PCon PTy PTm PTyEq PTmEq PTyConv PTmConv.
+  Proof.
+    subst PCon PTy PTm PTyEq PTmEq PTyConv PTmConv.
+    apply ParInduction.
+    all: try solve [trivial].
+    all: try solve [now econstructor].
+    intros.
+    eapply TermParApp ; refold ; tea.
+    now econstructor.
+  Qed.
+
+End LRefl.
+
+Section Congruences.
+
+  Lemma TermConvParVar Γ n n' decl :
+    [   |- Γ ] ->
+    in_ctx Γ n decl ->
+    n = n' ->
+    [ Γ |- tRel n ≅ tRel n' : decl ].
+  Proof.
+    intros ; subst.
+    now do 2 econstructor.
+  Qed.
+
+  Lemma TypeConvParProd Γ A A' B B' :
+    [Γ |- A ≅ A' ] ->
+    [Γ ,, A |- B ≅ B'] -> 
+    [ Γ |- tProd A B ≅ tProd A' B'].
+  Proof.
+    intros HA HB. 
+    induction HA in B, B', HB |- * ; refold.
+    - remember (Γ,,A) as Δ in HB.
+      induction HB ; refold.
+      + subst.
+        now do 2 econstructor.
+      + subst.
+        eapply TypeConvParL ; refold.
+        1: econstructor ; tea.
+        2: now eapply IHHB.
+        now eapply par_lrefl in t.
+      + now eapply IHHB.
+    - eapply TypeConvParL ; refold.
+  Abort.
+
+Section TypingWk.
+  
+  Let PCon (Γ : context) := True.
+  Let PTy (Γ : context) (A A' : term) := forall Δ (ρ : Δ ≤ Γ), [|- Δ ] -> [Δ |- A⟨ρ⟩ ⤳ A'⟨ρ⟩].
+  Let PTm (Γ : context) (A t t' : term) := forall Δ (ρ : Δ ≤ Γ), [|- Δ ] ->
+    [Δ |- t⟨ρ⟩ ⤳ t'⟨ρ⟩ : A⟨ρ⟩].
+  Let PTyEq (Γ : context) (A B : term) := forall Δ (ρ : Δ ≤ Γ), [|- Δ ] ->
+    [Δ |- A⟨ρ⟩ = B⟨ρ⟩].
+  Let PTmEq (Γ : context) (A t u : term) := forall Δ (ρ : Δ ≤ Γ), [|- Δ ] ->
+    [Δ |- t⟨ρ⟩ = u⟨ρ⟩ : A⟨ρ⟩].
+  Let PTyConv (Γ : context) (A B : term) := forall Δ (ρ : Δ ≤ Γ), [|- Δ ] ->
+    [Δ |- A⟨ρ⟩ ≅ B⟨ρ⟩].
+  Let PTmConv (Γ : context) (A t u : term) := forall Δ (ρ : Δ ≤ Γ), [|- Δ ] ->
+    [Δ |- t⟨ρ⟩ ≅ u⟨ρ⟩ : A⟨ρ⟩].
+
+  Theorem par_wk : ParInductionConcl PCon PTy PTm PTyEq PTmEq PTyConv PTmConv.
+  Proof.
+    subst PCon PTy PTm PTyEq PTmEq PTyConv PTmConv.
+    apply ParInduction.
+    all: try solve [now econstructor].
+    - intros * ? IHA ? IHB * ? ; cbn.
+      unshelve epose proof (IHA _ _ _) as IHA' ; tea.
+      econstructor ; eauto.
+      eapply IHB with (ρ := wk_up _ _).
+      econstructor ; tea.
+      now eapply par_lrefl in IHA'.
+    - intros ; cbn.
+      econstructor ; tea.
+      now eapply in_ctx_wk.
+    - intros * ? IHA ? IHB * ? ; cbn.
+      unshelve epose proof (IHA _ _ _) as IHA' ; tea.
+      econstructor ; eauto.
+      eapply IHB with (ρ := wk_up _ _).
+      econstructor ; tea.
+      econstructor.
+      now eapply par_lrefl in IHA'.
+    - intros * ? IHAconv ? IHAred ? IHt **.
+      unshelve epose proof (IHAred _ _ _) as IHA' ; tea.
+      cbn ; econstructor.
+      1-2: eauto.
+      eapply IHt with (ρ := wk_up _ _).
+      econstructor ; tea.
+      now eapply par_lrefl in IHA'.
+    - intros * ? IHAred ? IHAconv ? IHB ? IHt ? IHa **.
+      assert [Δ |- A⟨ρ⟩] by now eapply IHAred.
+      assert [Δ |- A'⟨ρ⟩] by (now unshelve epose proof (IHAconv _ _ _) as ?%par_lrefl).
+      cbn.
+      evar (B' : term) ; replace (B[_]⟨ρ⟩) with B' ; subst B'.
+      evar (t'' : term) ; replace (t'[_]⟨ρ⟩) with t'' ; subst t''.
+      1: econstructor ; eauto.
+      + now eapply IHB with (ρ := wk_up _ _) ; econstructor.
+      + now eapply IHt with (ρ := wk_up _ _) ; econstructor.
+      + now bsimpl.
+      + now bsimpl.
+    - intros * ? IHA ? IHA' ? IHB ? IHB' ? IHf ? IHa **.
+      assert [Δ |- A⟨ρ⟩] by now eapply IHA.
+      cbn.
+      evar (B'' : term) ; replace (B[_]⟨ρ⟩) with B'' ; subst B''.
+      1: econstructor ; eauto.
+      + now eapply IHB with (ρ := wk_up _ _) ; econstructor.
+      + now eapply IHB' with (ρ := wk_up _ _) ; econstructor.
+      + now bsimpl.
+    - intros * ? IHA ? IHB **.
+      cbn.
+      econstructor ; eauto.
+      eapply IHB with (ρ := wk_up _ _).
+      econstructor ; tea.
+      now eapply par_lrefl in IHA.
+    - intros **.
+      econstructor ; tea.
+      now eapply in_ctx_wk.
+    - intros * ? IHA ? IHB **.
+      cbn.
+      econstructor ; eauto.
+      eapply IHB with (ρ := wk_up _ _).
+      econstructor ; tea.
+      econstructor.
+      now eapply par_lrefl in IHA.
+    - intros * ? IHA ?? ? IHt **.
+      cbn.
+      econstructor ; eauto.
+      eapply IHt with (ρ := wk_up _ _).
+      econstructor ; tea.
+      now eapply par_lrefl in IHA.
+    - intros * ? IHA ? IHB ? IHf ? IHa **.
+      cbn.
+      evar (B'' : term) ; replace (B[_]⟨ρ⟩) with B'' ; subst B''.
+      1: econstructor ; eauto.
+      + eapply IHB with (ρ := wk_up _ _) ; econstructor ; tea.
+        now eapply par_lrefl in IHA.
+      + now bsimpl.
+  Qed.
+
+End TypingWk.
